Vegas/Machine.lean
@@ -50,6 +50,7 @@ import Vegas.Machine.Contract.Imperative
 import Vegas.Machine.Contract.ClassicalEVMCodegen
 import Vegas.Machine.Contract.ClassicalEVMCodegenCorrect
 import Vegas.Machine.Contract.SimpleEVMExpr
+import Vegas.Machine.Contract.SimpleEVMExprCorrect
 import Vegas.Machine.Contract.SimpleEVMAction
 import Vegas.Machine.Contract.SimpleEVMDist
 import Vegas.Machine.Contract.SimpleEVMSample
